Spec of addrspace execution looks plausible

verified/entry.s.dfy
@@ -2,17 +2,103 @@ include "kev_common.s.dfy"
 include "ARMdef.dfy"
 include "pagedb.s.dfy"
 include "smcapi.s.dfy"
-
-//TODO refactor this since trusted files should not include untrusted files
 include "pagedb.i.dfy"
-include "entry.i.dfy"
 
 predicate entryState(s:state, d:PageDb)
 {
     reveal_validPageDb();
     ValidState(s) && SaneMem(s.m) && validPageDb(d) &&
     (validPageDbImpliesClosedRefs(d); pageDbCorresponds(s.m, d)) &&
-    validL1PTPage(d, s.conf.l1p) && !stoppedAddrspace(d, s.conf.l1p)
+    validL1PTPage(d, s.conf.l1p) && !stoppedAddrspace(d, s.conf.l1p) &&
+    s.conf.m == User && s.conf.ns == Secure
+}
+
+predicate validEntryTransition(s:state,s':state,d:PageDb,d':PageDb,
+    dispPage:PageNr,a1:int,a2:int,a3:int)
+    requires isUInt32(a1) && isUInt32(a2) && isUInt32(a3) 
+    requires ValidState(s) && SaneMem(s.m) && validPageDb(d)
+    requires (validPageDbImpliesClosedRefs(d); pageDbCorresponds(s.m, d))
+    requires smc_enter(d, dispPage, a1, a2, a3).1 == KEV_ERR_SUCCESS()
+{
+    //reveal_validConfig();
+    reveal_validPageDb();
+    reveal_ValidConfig();
+	var addrspace := d[d[dispPage].addrspace].entry;
+    s'.conf.m  == User && s'.conf.ns == Secure && s'.conf.l1p == addrspace.l1ptnr &&
+    OSymbol("g_cur_dispatcher") in s'.m.globals &&
+    s'.m.globals[OSymbol("g_cur_dispatcher")] == [dispPage] &&
+    entryState(s', d') &&
+    d' == d && pageDbCorresponds(s'.m, d')
+}
+
+predicate validReturnTransition(s:state,s':state,d:PageDb,d':PageDb)
+{
+    // The following specifies that this is the return path after execution
+        // q is the state immediately upon entry.
+        // r is the state just before calling the exception handler.
+    (exists q, r :: entryState(q, d) && userspaceExecution(q, r, d) &&
+        exception(r, s, d, d')) &&
+
+    // leave secure world
+    s'.conf.ns == NotSecure
+}
+
+predicate svc(s:state,s':state,d:PageDb,d':PageDb) 
+{
+    // TODO disable interrupts (cpsid is called in impl)
+    entryState(s, d) && entryState(s', d') && s'.conf.m == Monitor &&
+    d' == d &&
+    s'.regs[R0] == KEV_ERR_SUCCESS()
+}
+
+predicate irqfiq(s:state,s':state,d:PageDb,d':PageDb)
+{
+    
+    entryState(s, d) && entryState(s', d') && s'.conf.m == Monitor &&
+    s'.regs[R0] == KEV_ERR_INTERRUPTED() &&
+    
+    (var dispPage := s.m.globals[OSymbol("g_cur_dispatcher")][0];
+    var a := d[ dispPage ].addrspace;
+    var disp := d[dispPage].entry;
+    d'[dispPage] == PageDbEntryTyped(a,
+        Dispatcher(disp.entrypoint, true, s.regs))) &&
+
+    // Interrupts can be taken from other modes, but the interrupt should
+    // only re-enter monitor mode when taken from user mode.
+    // This spec is intended to be used with an irq/fiq handler that
+    // calls separate procedures for the from-user and not-from-user case.
+    // Only the from-user case satisfies this predicate.
+    s.conf.spsr[s.conf.m] == User
+    
+}
+
+predicate abort(s:state,s':state,d:PageDb,d':PageDb)
+{
+    // TODO disable interrupts (cpsid is called in impl)
+    entryState(s, d) && entryState(s', d') && s'.conf.m == Monitor &&
+
+    (var dispPage := s.m.globals[OSymbol("g_cur_dispatcher")][0];
+    var a := d[ dispPage ].addrspace;
+    var disp := d[dispPage].entry;
+    d'[dispPage] == PageDbEntryTyped(a, Dispatcher(disp.entrypoint, true, s.regs))) &&
+
+    s'.regs[R0] == KEV_ERR_FAULT()
+}
+
+//-----------------------------------------------------------------------------
+// Userspace Execution
+//-----------------------------------------------------------------------------
+
+//The code executing in userspace is possibly malicious. This models its limitations.
+predicate userspaceExecution(s:state, s':state, d:PageDb)
+{
+    entryState(s, d) && WSMemInvariantExceptAddrspace(s, s', d) &&
+    entryState(s', d)
+}
+
+predicate exception(s:state, s':state, d:PageDb, d':PageDb)
+{
+    svc(s,s',d,d') || irqfiq(s,s',d,d') || abort(s,s',d,d')
 }
 
 // All writeable and secure memory addresses except the ones in the active l1
@@ -55,92 +141,35 @@ predicate pageSWrInL2PT(l2pt:seq<L2PTE>, p:PageNr)
         case InsecureMapping(p') => false)
 }
 
-//-----------------------------------------------------------------------------
-// Assumptions about user mode execution of the addrspace
-//-----------------------------------------------------------------------------
-function {:axiom} addrspaceHavoc(s:state, d:PageDb) : state
-    requires entryState(s, d)
-    ensures var s' := addrspaceHavoc(s, d);
-        WSMemInvariantExceptAddrspace(s, s', d) && SaneMem(s'.m) &&
-        s'.conf == s.conf
 
-function {:axiom} addrspaceReturn(s:state, d:PageDb) : state
-    requires entryState(s, d)
-    ensures 
-        addrspaceReturn(s, d) == svc(s)   ||
-        addrspaceReturn(s, d) == irq(s)   ||
-        addrspaceReturn(s, d) == fiq(s)   ||
-        addrspaceReturn(s, d) == abort(s)
-
-
-//-----------------------------------------------------------------------------
-// Addrspace entry / return path
-//-----------------------------------------------------------------------------
-
-function entry(s:state, disp: PageNr, a1: int, a2: int, a3: int, d:PageDb) : state
-    requires entryState(s, d)
-    // TODO requires pageDbCorresponds
-{
-    var s1 := enterDispatchFunctional(s, disp, a1, a2, a3, d);
-    assume false; // TODO need premium enterDispatchFunctional
-    var s2 := addrspaceHavoc(s1, d);
-    var s3 := addrspaceReturn(s2, d);
-    s3
-}
-
-//-----------------------------------------------------------------------------
-// Safety poperties of the monitor/addrspace boundary
-//-----------------------------------------------------------------------------
-
-// The pages owned by other addrspaces are preserved
-predicate {:opaque} addrspaceContentsPreservedExcept(s:state, s':state, disp:PageNr, d: PageDb)
-    requires entryState(s, d)
-    requires validDispatcherPage(d, disp)
-{
-    reveal_validPageDb();
-    var a := d[disp].addrspace;
-    ValidState(s') && AlwaysInvariant(s, s') &&
-    forall a' :: validAddrspacePage(d, a') && a' != a && !stoppedAddrspace(d, a') ==>
-        (var l1' := d[a'].entry.l1ptnr;
-        forall m :: memSWrInAddrspace(d, l1', m) ==>
-            s.m.addresses[m] == s'.m.addresses[m])
-}
-
-// // Probaby needed to prove next lemma
-// lemma addrspaceHavocPreservesPageDb(s:state, d:PageDb)
-//     requires entryState(s, d)
-//     ensures var s' := addrspaceHavoc(s, d);
-//         (validPageDbImpliesClosedRefs(d); pageDbCorresponds(s'.m, d))
+// Copied from old entry.s.dfy
+// //-----------------------------------------------------------------------------
+// // Safety poperties of the monitor/addrspace boundary
+// //-----------------------------------------------------------------------------
+// 
+// predicate addrspaceOwnershipOfPagesPreserved(d:PageDb, d':PageDb)
+//     // requires entryState(s, d) && entryState(s', d')
+//     requires validPageDb(d) && validPageDb(d')
 // {
-//     //TODO PROVEME
-// 	assume false;
+//     reveal_validPageDb();
+//     forall a :: validAddrspacePage(d, a) ==>
+//         validAddrspacePage(d', a) && 
+//         (var l1 := d[a].entry.l1ptnr;
+//         forall m :: !stoppedAddrspace(d,a) && memSWrInAddrspace(d, l1, m) ==> 
+//             d'[a] == d[a] && !stoppedAddrspace(d', a) && memSWrInAddrspace(d', l1, m))
 // }
 // 
-// lemma addrspaceExecutePreservesPageDb(s:state, d:PageDb)
-//     requires entryState(s, d)
-//     ensures var s' := addrspaceExecute(s, d, a);
-//         (validPageDbImpliesClosedRefs(d); pageDbCorresponds(s'.m, d))
+// // The pages owned by other addrspaces are preserved
+// predicate addrspaceContentsPreservedExcept(s:state, s':state, d: PageDb, d':PageDb, disp:PageNr)
+//     requires entryState(s, d) && entryState(s', d')
+//     requires addrspaceOwnershipOfPagesPreserved(d, d')
+//     requires valid
 // {
-//     //TODO PROVEME
-// 	assume false;
+//     reveal_validPageDb();
+//     var a := d[disp].addrspace;
+//     ValidState(s') && AlwaysInvariant(s, s') &&
+//     forall a' :: validAddrspacePage(d, a') && a' != a && !stoppedAddrspace(d, a') ==>
+//         (var l1' := d[a'].entry.l1ptnr;
+//         forall m :: memSWrInAddrspace(d, l1', m) ==>
+//             s.m.addresses[m] == s'.m.addresses[m])
 // }
-
-
-lemma entryPreservesOtherAddrspaces(s:state, disp:PageNr, a1:int, a2:int, a3:int, d:PageDb)
-    requires entryState(s, d)
-    ensures  validDispatcherPage(d, disp)
-    ensures  var s' := entry(s, disp, a1, a2, a3, d);
-        addrspaceContentsPreservedExcept(s, s', disp, d)
-{
-    //TODO prove 
-    assume false;
-}
-
-
-//-----------------------------------------------------------------------------
-// Liveness Properties of the monitor/addrspace bondary
-//-----------------------------------------------------------------------------
-
-// The sequence enter -> execute -> return -> enter -> execute restores the
-    // context from the first execute?
-
